15 apply-style proofs left

SimPro.thy
@@ -132,44 +132,40 @@ lemma patom:  "(n,(m,Pos i v) # xs) \<in> calculation(nfs) \<Longrightarrow> \<n
   and fdisj:  "(n,(m,Dis f g) # xs) \<in> calculation(nfs) \<Longrightarrow> \<not> is_axiom (list_sequent ((m,Dis f g) # xs)) \<Longrightarrow> (Suc n,xs@[(0,f),(0,g)]) \<in> calculation(nfs)"
   and fall:   "(n,(m,Uni f) # xs) \<in> calculation(nfs) \<Longrightarrow> \<not> is_axiom (list_sequent ((m,Uni f) # xs)) \<Longrightarrow> (Suc n,xs@[(0,substitution_bind f (fresh ((flatten \<circ> map fv) (list_sequent ((m,Uni f) # xs)))))]) \<in> calculation(nfs)"
   and fex:    "(n,(m,Exi f) # xs) \<in> calculation(nfs) \<Longrightarrow> \<not> is_axiom (list_sequent ((m,Exi f) # xs)) \<Longrightarrow> (Suc n,xs@[(0,substitution_bind f m),(Suc m,Exi f)]) \<in> calculation(nfs)"
-  by (auto simp add: inference_def list_sequent_def comp_def)
+  by (auto simp: inference_def list_sequent_def comp_def)
 
 lemmas not_is_axiom_subs = patom natom fconj1 fconj2 fdisj fall fex
 
 lemma calculation0[simp]: "(0,x) \<in> calculation y = (x = y)"
   using calculation.cases by blast
 
-lemma calculation_upwards: "(n,list) \<in> calculation s \<Longrightarrow> \<not> is_axiom (list_sequent (list)) \<Longrightarrow> (\<exists>zs. (Suc n, zs) \<in> calculation s \<and> zs : set (inference list))"
-  using inference_def list_sequent_def by (case_tac list, fastforce, case_tac a, case_tac b, force+)
+lemma calculation_upwards:
+  assumes 1: "(n,x) \<in> calculation s" and 2: "\<not> is_axiom (list_sequent (x))"
+  shows "(\<exists>y. (Suc n, y) \<in> calculation s \<and> y : set (inference x))"
+  proof (cases x)
+    case Nil then show ?thesis using 1 inference_def by auto
+  next
+    case c: (Cons a _) then show ?thesis
+    proof (cases a)
+      case (Pair _ p)
+      then show ?thesis using c 1 2 list_sequent_def inference_def by (cases p) (auto, fastforce)
+    qed
+  qed
 
 lemma calculation_downwards: "(Suc n, x) \<in> calculation s \<Longrightarrow> \<exists>y. (n,y) \<in> calculation s \<and> x : set (inference y) \<and> \<not> is_axiom (list_sequent y)"
-  apply(erule calculation.cases)
-  apply(simp)
-  apply(simp add: list_sequent_def Let_def)
-  apply(rule_tac x=k in exI) apply(simp)
-  apply(case_tac k) apply(simp)
-  apply(case_tac a) apply(case_tac b) 
-       apply(auto simp add: Let_def)
-   apply (rename_tac[!] nat lista a)
-apply(simp only: list_sequent_def inference_def)
-   apply(subgoal_tac "Neg nat lista \<in> snd ` set list") apply(simp) apply(force)
-  apply(subgoal_tac "Pos nat lista \<in> snd ` set list")
-apply(simp only: list_sequent_def inference_def)
-apply(simp) apply(force)
-  done
-
+  by (erule calculation.cases, simp_all add: list_sequent_def, rule exI, case_tac k, fastforce, case_tac a, case_tac b)
+     (fastforce simp: inference_def list_sequent_def)+
+ 
 lemma calculation_calculation_child[rule_format]: "\<forall>x y. (Suc n,x) \<in> calculation y = (\<exists>z. z : set (inference y) \<and> \<not> is_axiom (list_sequent y) \<and> (n,x) \<in> calculation z)"
-  apply(induct n)
-   apply(rule, rule) apply(rule) apply(frule_tac calculation_downwards) apply(simp)
-   apply(simp) apply(rule step) apply(simp) apply(simp)
-  apply(blast dest!: calculation_downwards elim: calculation.cases) -- "blast needs some help with the reasoning, hence calculationSucE"
-  done
+  using calculation_downwards by (induct n) (fastforce, blast)
 
-lemma calculation_progress: "(n,a # list) \<in> calculation s \<Longrightarrow> \<not> is_axiom (list_sequent (a # list)) \<Longrightarrow> (\<exists>zs. (Suc n, list@zs) \<in> calculation s)"
-  apply(subgoal_tac "a # list \<noteq> []") prefer 2 apply(simp)
-  apply(case_tac a) apply(case_tac b)
-       apply(force dest: not_is_axiom_subs)+
-  done
+lemma calculation_progress:
+  assumes 1:  "(n,a # list) \<in> calculation s" and 2: "\<not> is_axiom (list_sequent (a # list))"
+  shows "(\<exists>zs. (Suc n, list@zs) \<in> calculation s)"
+  proof (cases a)
+    case p: (Pair _ p)
+    show ?thesis using p 1 2 by (cases p) (auto dest: not_is_axiom_subs)
+  qed
 
 definition
   inc :: "nat \<times> sequent \<Rightarrow> nat \<times> sequent" where
@@ -178,21 +174,13 @@ definition
 lemma inj_inc[simp]: "inj inc"
   by (simp add: inc_def inj_on_def)
 
-lemma calculation: "calculation y = insert (0,y) (inc ` (Union (calculation ` {w. \<not> is_axiom (list_sequent y) \<and> w : set (inference y)})))"
-  apply(rule set_eqI)
-  apply(simp add: split_paired_all)
-  apply(case_tac a)
-   apply(force simp: inc_def)
-  apply(force simp: calculation_calculation_child inc_def)
-  done
+lemma calculation: "calculation y = insert (0,y) (inc ` (\<Union> (calculation ` {w. \<not> is_axiom (list_sequent y) \<and> w : set (inference y)})))"
+   by (rule set_eqI, simp add: split_paired_all, case_tac a)
+     (auto simp: calculation_calculation_child inc_def)+
 
 lemma calculation_is_axiom: "is_axiom (list_sequent s) \<Longrightarrow> calculation s = {(0,s)}"
-  apply(rule)
-   apply(rule)
-   apply(case_tac x) apply(simp)
-   apply(erule_tac calculation.induct) apply(force) apply(simp_all add: list_sequent_def) apply(case_tac s) apply(simp) apply(case_tac aa) apply(case_tac ba)
-         apply(simp_all add: list_sequent_def inference_def)
-  done
+  by (rule set_eqI, rule iffI, intro insertCI)
+     (metis calculation.simps calculation_calculation_child prod.exhaust, blast)
    
 lemma is_axiom_finite_calculation: "is_axiom (list_sequent s) \<Longrightarrow> finite (calculation s)"
   by (simp add: calculation_is_axiom)
@@ -211,13 +199,13 @@ lemma infinite_union: "finite Y \<Longrightarrow> infinite (Union (f ` Y)) \<Lon
   by auto
 
 lemma infinite_inj_infinite_image: "inj_on f Z \<Longrightarrow> infinite (f ` Z) = infinite Z"
-  by (auto dest: finite_imageD)
+  using finite_imageD by auto
 
 lemma inj_inj_on: "inj f \<Longrightarrow> inj_on f A"
-  by (blast intro: subset_inj_on)
+  using subset_inj_on by blast
 
 lemma t: "finite {w. P w} \<Longrightarrow> finite {w. Q w \<and> P w}"
-  by (simp add: finite_subset)
+  using finite_subset by simp
 
 lemma finite_subs: "finite {w. \<not> is_axiom (list_sequent y) \<and> w : set (inference y)}"
   by simp
@@ -225,23 +213,26 @@ lemma finite_subs: "finite {w. \<not> is_axiom (list_sequent y) \<and> w : set (
 lemma (in loc1) fSuc: "f n \<in> calculation s \<and> fst (f n) = n \<and> infinite (calculation (snd (f n))) \<and> \<not> is_axiom (list_sequent (snd (f n)))
   \<Longrightarrow> f (Suc n) \<in> calculation s \<and> fst (f (Suc n)) = Suc n \<and> (snd (f (Suc n))) : set (inference (snd (f n))) \<and> infinite (calculation (snd (f (Suc n)))) \<and> \<not> is_axiom (list_sequent (snd (f (Suc n))))"
   apply(simp add: f)
-  apply(rule_tac someI_ex)
-  apply(simp only: f[symmetric]) 
-  apply(drule_tac subst[OF calculation[of "snd (f n)"] ])
-  apply(simp only: finite_insert) apply(subgoal_tac "infinite (\<Union>(calculation ` {w. \<not> is_axiom (list_sequent (snd (f n))) \<and> w : set (inference (snd (f n)))}))")
-   apply(drule_tac infinite_union[OF finite_subs]) apply(erule exE) apply(rule_tac x="(Suc n, y)" in exI)
-   apply(clarify) apply(simp) apply(case_tac "f n") apply(simp add: step) apply(force simp add: is_axiom_finite_calculation)
-  apply(force simp add: infinite_inj_infinite_image inj_inj_on) 
+  apply(rule someI_ex)
+  apply(simp only: f[symmetric])
+  apply(drule subst[OF calculation[of "snd (f n)"] ])
+  apply(subgoal_tac "infinite (\<Union>(calculation ` {w. \<not> is_axiom (list_sequent (snd (f n))) \<and> w : set (inference (snd (f n)))}))")
+   apply(drule infinite_union[OF finite_subs])
+   apply(erule exE)
+   apply(rule exI)
+   apply(cases "f n")
+   apply(fastforce simp: is_axiom_finite_calculation)
+  apply(fastforce simp: infinite_inj_infinite_image inj_inj_on)
   done
 
 lemma (in loc1) is_path_f_0: "infinite (calculation s) \<Longrightarrow> f 0 = (0,s)"
-  by (metis calculation0 f0 prod.collapse)
+  using calculation0 f0 prod.collapse by metis
 
 lemma (in loc1) is_path_f': "infinite (calculation s) \<Longrightarrow> f n \<in> calculation s \<and> fst (f n) = n \<and> infinite (calculation (snd (f n))) \<and> \<not> is_axiom (list_sequent (snd (f n)))"
-  by (induct n) (auto simp add: f0 fSuc)
+  using f0 fSuc by (induct n) auto
 
 lemma (in loc1) is_path_f: "infinite (calculation s) \<Longrightarrow> \<forall>n. f n \<in> calculation s \<and> fst (f n) = n \<and> (snd (f (Suc n))) : set (inference (snd (f n))) \<and> infinite (calculation (snd (f n)))"
-  by (simp add: is_path_f' fSuc)
+  using is_path_f' fSuc by simp
 
 lemma ball_eq_ball: "\<forall>x \<in> m. P x = Q x \<Longrightarrow> (\<forall>x \<in> m. P x) = (\<forall>x \<in> m. Q x)"
   by blast
@@ -249,24 +240,29 @@ lemma ball_eq_ball: "\<forall>x \<in> m. P x = Q x \<Longrightarrow> (\<forall>x
 lemma bex_eq_bex: "\<forall>x \<in> m. P x = Q x \<Longrightarrow> (\<exists>x \<in> m. P x) = (\<exists>x \<in> m. Q x)"
   by blast
 
-lemma cut[simp]:"Suc n \<in> set A = (n \<in> set (cut A))"
-  by (induct A) (simp, case_tac a, simp_all)
+lemma cut[simp]: "Suc n \<in> set A = (n \<in> set (cut A))"
+  proof (induct A)
+    case Nil then show ?case by simp
+  next
+    case (Cons m _) then show ?case by (cases m) simp_all
+  qed
 
 lemma FEval_cong: "\<forall>e1 e2. (\<forall>xx. xx \<in> set (fv A) \<longrightarrow> e1 xx = e2 xx) \<longrightarrow> semantics mi e1 A = semantics mi e2 A"
-  apply(induct_tac A)
-       apply(simp add: Let_def) apply(intro allI impI) apply(rule arg_cong, rule map_cong) apply(rule) apply(force)
-     apply(simp add: Let_def) apply(intro allI impI) apply(rule conj_cong) apply(force) apply(force)
-   apply(simp add: Let_def) apply(intro allI impI) apply(rule ball_eq_ball) apply(rule) 
-   apply(drule_tac x="case_nat z e1" in spec) apply(drule_tac x="case_nat z e2" in spec) apply(erule impE)
-    apply(rule) apply(rule) apply(rename_tac x) apply(case_tac x) apply(simp) apply(simp)
-   apply(assumption)
-      apply(simp add: Let_def) apply(intro allI impI) apply(rule arg_cong, rule map_cong) apply(rule)  apply(force)
-    apply(simp add: Let_def) apply(intro allI impI) apply(rule disj_cong) apply(force) apply(force)
-  apply(simp add: Let_def) apply(intro allI impI) apply(rule bex_eq_bex) apply(rule)
-  apply(drule_tac x="case_nat z e1" in spec) apply(drule_tac x="case_nat z e2" in spec) apply(erule impE)
-   apply(rule) apply(rule) apply(rename_tac x) apply(case_tac x) apply(simp) apply(simp)
-  apply(assumption)
-  done
+  proof (induct A)
+    case Pos then show ?case using map_cong fv.simps(1) semantics.simps(1) by metis
+  next
+    case Neg then show ?case using map_cong fv.simps(2) semantics.simps(2) by metis
+  next
+    case Con then show ?case using Un_iff fv.simps(3) semantics.simps(3) set_append by metis
+  next
+    case Dis then show ?case using  Un_iff fv.simps(4) semantics.simps(4) set_append by metis
+  next
+    case Uni then show ?case
+      by(clarsimp, intro ball_eq_ball) (metis (no_types, lifting) Nitpick.case_nat_unfold Suc_pred' cut not_gr0)
+  next
+    case Exi then show ?case
+      by (clarsimp, intro bex_eq_bex) (metis (no_types, lifting) Nitpick.case_nat_unfold Suc_pred' cut not_gr0)
+  qed
 
 lemma semantics_alternative_def2: "semantics_alternative m e s = (\<exists>p. p \<in> set s \<and> semantics m e p)"
   by (induct s) auto
@@ -280,103 +276,71 @@ lemma fv_list_nil: "fv_list [] = []"
 lemma fv_list_cons: "fv_list (a # list) = (fv a) @ (fv_list list)"
   by (simp add: fv_list_def)
 
-lemma semantics_alternative_cong: "(\<forall>x. x \<in> set (fv_list s) \<longrightarrow> e1 x = e2 x) \<longrightarrow> semantics_alternative m e1 s = semantics_alternative m e2 s"
-  by (induct s) (simp, metis FEval_cong semantics_alternative.simps(2) Un_iff set_append fv_list_cons)
+lemma semantics_alternative_cong: "(\<forall>x. x \<in> set (fv_list s) \<longrightarrow> e1 x = e2 x) \<longrightarrow> semantics_alternative m e1 s = semantics_alternative m e2 s" 
+ by (induct s) (simp, metis FEval_cong semantics_alternative.simps(2) Un_iff set_append fv_list_cons)
 
 section "Soundness"
 
 lemma FEval_substitution: "\<forall>e f. (semantics mi e (substitution f A)) = (semantics mi (e \<circ> f) A)"
-  apply(induct A)
-       apply(simp add: Let_def) apply(simp only: comp_def) apply(blast)
-    apply(simp)
-   apply(simp) apply(rule,rule) apply(rule ball_eq_ball) apply(rule)
-   apply(subgoal_tac "(\<lambda>u. case_nat z e (case u of 0 \<Rightarrow> 0 | Suc n \<Rightarrow> Suc (f n))) = (case_nat z (\<lambda>n. e (f n)))") apply(simp)
-   apply(rule ext) apply(case_tac u)
-    apply(simp) apply(simp)
-      apply(simp add: Let_def) apply(simp only: comp_def) apply(blast)
-     apply(simp)
-  apply(simp) apply(rule,rule) apply(rule bex_eq_bex) apply(rule)
-  apply(subgoal_tac "(\<lambda>u. case_nat z e (case u of 0 \<Rightarrow> 0 | Suc n \<Rightarrow> Suc (f n))) = (case_nat z (\<lambda>n. e (f n)))") apply(simp)
-  apply(rule ext) apply(case_tac u)
-   apply(simp) apply(simp)
-  done
+  proof (induct A)
+    case Pos then show ?case by (simp add: comp_def)
+  next
+    case Neg then show ?case by (simp add: comp_def)
+  next
+    case Con then show ?case by (simp add: comp_def)
+  next
+    case Dis then show ?case by (simp add: comp_def)
+  next
+    case Uni then show ?case
+      by (clarsimp, intro ball_eq_ball) (simp add: FEval_cong Nitpick.case_nat_unfold)
+  next
+    case Exi then show ?case
+      by (clarsimp, intro bex_eq_bex) (simp add: FEval_cong Nitpick.case_nat_unfold)
+  qed
 
 lemma FEval_substitution_bind: "semantics mo e (substitution_bind A u) = semantics mo (case_nat (e u) e) A"
-  apply(simp add: substitution_bind_def)
-  apply(simp add: FEval_substitution)
-  apply(subgoal_tac "(e \<circ> case_nat u (\<lambda>n. n)) = (case_nat (e u) e)") apply(simp)
-  apply(rule ext)
-  apply(case_tac x, auto)
-  done
+  using substitution_bind_def FEval_substitution FEval_cong
+  by (simp add: Nitpick.case_nat_unfold)
 
 lemma ball_maxscope: "(\<forall>x \<in> m. P x \<or> Q) \<Longrightarrow> (\<forall>x \<in> m. P x) \<or> Q "
   by simp
 
 lemma sound_FAll: "u \<notin> set (fv_list (Uni f # s)) \<Longrightarrow> valid (s@[substitution_bind f u]) \<Longrightarrow> valid (Uni f # s)"
-  apply(simp add: valid_def del: semantics_alternative.simps)
-  apply(rule allI) 
+  apply(simp add: valid_def)
+  apply(rule allI)
   apply(rule allI)
   apply(rename_tac M I)
-  apply(rule allI) apply(rule)
-  apply(simp add: semantics_alternative_append)
-  apply(rule ball_maxscope)
-  apply(rule)
-  apply(simp add: FEval_substitution_bind)
+  apply(clarsimp simp: semantics_alternative_append FEval_substitution_bind)
 
   apply(drule_tac x=M in spec, drule_tac x=I in spec) -- "this is the goal"
 
-  apply(drule_tac x="e(u:=z)" in spec) apply(erule impE) apply(simp add: is_model_environment_def) apply(erule disjE)
-   apply(rule disjI2)
+  apply(drule_tac x="e(u:=z)" in spec)
+  apply(erule impE)
+   apply(simp add: is_model_environment_def)
+  apply(erule disjE)
    apply(subgoal_tac "semantics_alternative (M,I) (e(u:=z)) s = semantics_alternative (M,I) e s")
     apply(simp)
-   apply(rule semantics_alternative_cong[rule_format]) apply(simp add: fv_list_cons) apply(force)
-
-  apply(rule disjI1)
-  apply(simp)
+   apply(rule semantics_alternative_cong[rule_format])
+   apply(clarsimp simp: fv_list_cons)
+  
   apply(subgoal_tac "semantics (M,I) (case_nat z (e(u:=z))) f = semantics (M,I) (case_nat z e) f")
    apply(simp)
   apply(rule FEval_cong[rule_format])
 
-  apply(case_tac xx, simp)
-  apply(simp only: cut[rule_format, symmetric])
-  apply(subgoal_tac "nat \<in> set (fv (Uni f))") prefer 2 apply(simp)
-  
-  apply(force simp: fv_list_cons)
+  apply(case_tac xx)
+    apply(simp)
+  apply(clarsimp simp: fv_list_cons)
   done
     -- "phew, that really was a bit more difficult than expected"
     -- "note that we can avoid maxscoping at the cost of instantiating the hyp twice- an additional time for M"
     -- "different proof, instantiating quantifier twice, avoiding maxscoping --- not much better, probably slightly worse"
 
 lemma sound_FEx: "valid (s@[substitution_bind f u,Exi f]) \<Longrightarrow> valid (Exi f # s)"
-  apply(simp add: valid_def del: semantics_alternative.simps)
-  apply(rule allI)
-  apply(rule allI)
-  apply(rename_tac ms m)
-  apply(rule) apply(rule)
-  apply(simp add: semantics_alternative_append FEval_substitution_bind)
-
-  apply(drule_tac x=ms in spec, drule_tac x=m in spec)
-  apply(drule_tac x=e in spec) apply(erule impE) apply(assumption)
-  apply(erule disjE)
-  apply(simp)
-  apply(erule disjE)
-   apply(rule disjI1)
-   apply(rule_tac x="e u" in bexI) apply(simp) apply(simp add: is_model_environment_def)
-  apply(force)
-  done
+  by (simp add: valid_def semantics_alternative_append FEval_substitution_bind)
+     (metis is_model_environment_def prod.sel(1))
 
 lemma max_exists: "finite (X::nat set) \<Longrightarrow> X \<noteq> {} \<longrightarrow> (\<exists>x. x \<in> X \<and> (\<forall>y. y \<in> X \<longrightarrow> y \<le> x))"
-  apply(erule_tac finite_induct) 
-  apply(force)
-  apply(rule)
-  apply(case_tac "F = {}")
-  apply(force)
-  apply(erule impE) apply(force)
-  apply(elim exE conjE)
-  apply(rule_tac x="max x xa" in exI)
-  apply(rule) apply(simp add: max_def)
-  apply(simp add: max_def) apply(force)
-  done -- "poor max lemmas in lib"
+  using Max.coboundedI Max_in by blast
 
 lemma inj_finite_image_eq_finite: "inj_on f Z \<Longrightarrow> finite (f ` Z) = finite Z"
   using finite_imageD by blast
@@ -391,169 +355,203 @@ definition init :: "sequent \<Rightarrow> bool" where
   "init s = (\<forall>x \<in> (set s). fst x = 0)"
 
 definition is_FEx :: "form \<Rightarrow> bool" where
-  "is_FEx f = (case f of 
-      Pos i v \<Rightarrow> False
-    | Neg i v \<Rightarrow> False
-    | Con f g \<Rightarrow> False
-    | Dis f g \<Rightarrow> False
-    | Uni f \<Rightarrow> False
-    | Exi f \<Rightarrow> True)"
+  "is_FEx f = (case f of
+    Exi _ \<Rightarrow> True |
+    _     \<Rightarrow> False)"
 
 lemma is_FEx[simp]: "\<not> is_FEx (Pos i v) \<and> \<not> is_FEx (Neg i v) \<and> \<not> is_FEx (Con f g) \<and> \<not> is_FEx (Dis f g) \<and> \<not> is_FEx (Uni f)"
-  by (simp add: is_FEx_def)
+  using is_FEx_def by simp
 
 lemma index0: "init s \<Longrightarrow> \<forall>u m A. (n, u) \<in> calculation s \<longrightarrow> (m,A) \<in> (set u) \<longrightarrow> (\<not> is_FEx A) \<longrightarrow> m = 0"
-  apply(induct_tac n)
-  apply(rule,rule,rule,rule,rule,rule) apply(simp) apply(force simp add: init_def)
-  apply(rule,rule,rule,rule,rule,rule)
+  apply(induct n)
+   apply(fastforce simp: init_def)
+  apply(clarsimp)
   -- {*inversion on @{term "(Suc n, u) \<in> calculation s"}*}
-  apply(drule_tac calculation_downwards) apply(elim exE conjE)
-  apply(case_tac y) apply(simp add: inference_def)
-  apply(case_tac a) apply(case_tac b)
-       apply(force simp add: list_sequent_def inference_def)
-      apply(force simp add: list_sequent_def inference_def)
-     apply(force simp add: list_sequent_def inference_def)
-    apply(force simp add: list_sequent_def inference_def)
-   apply(force simp add: list_sequent_def inference_def)
-  apply(force simp add: is_FEx_def list_sequent_def inference_def)
+  apply(drule calculation_downwards)
+  apply(elim exE)
+  apply(case_tac y)
+   apply(simp add: inference_def)
+  apply(case_tac a)
+  apply(case_tac b)
+        apply(fastforce simp: is_FEx_def list_sequent_def inference_def)+
   done
 
 lemma max_list: "\<forall>v \<in> set l. v \<le> max_list l"
-  by (induct l) (auto simp add: max_def)
+  by (induct l) (auto simp: max_def)
 
 lemma fresh: "fresh l \<notin> (set l)"
-  using length_pos_if_in_set max_list fresh_def by force
+  using length_pos_if_in_set max_list fresh_def by fastforce
 
 lemma soundness': "init s \<Longrightarrow> finite (calculation s) \<Longrightarrow> m \<in> (fst ` (calculation s)) \<Longrightarrow> \<forall>y u. (y,u) \<in> (calculation s) \<longrightarrow> y \<le> m \<Longrightarrow> \<forall>n t. h = m - n \<and> (n,t) \<in> calculation s \<longrightarrow> valid (list_sequent t)"
-using inference_def fv_list_def
+  using inference_def fv_list_def
   apply(induct_tac h)
     -- "base case"
-   apply(simp) apply(rule,rule,rule) apply(elim conjE)
-   apply(subgoal_tac "n=m") prefer 2 apply(force)
-   apply(simp)
-   apply(simp add: valid_def) apply(rule,rule) apply(rename_tac gs g) apply(rule) apply(rule) apply(simp add: semantics_alternative_def2)
+   apply(rule allI, rule allI, rule impI)
+   apply(elim conjE)
+    apply(subgoal_tac "n=m") prefer 2
+    apply(fastforce)
+   apply(simp add: valid_def)
+   apply(rule allI, rule allI)
+   apply(rename_tac gs g)
+   apply(rule allI)
+   apply(rule impI)
+   apply(simp add: semantics_alternative_def2)
    apply(case_tac "is_axiom (list_sequent t)")
      -- "base case, is axiom"
-    apply(simp add: list_sequent_def) apply(case_tac t) apply(simp) apply(simp)
+    apply(simp add: list_sequent_def)
+    apply(case_tac t)
+     apply(simp)
+    apply(simp)
     apply(erule disjE) 
       -- "base case, is axiom, starts with Pos"
-     apply(elim conjE exE)
-     apply(subgoal_tac "semantics (gs,g) e (Pos i v) \<or> semantics (gs,g) e (Neg i v)")
-      apply(erule disjE) apply(force) apply(rule_tac x="Neg i v" in exI) apply(force)
-     apply(simp add: Let_def)
-      -- "base case, is axiom, starts with Neg"
-    apply(elim conjE exE)
-    apply(subgoal_tac "semantics (gs,g) e (Pos i v) \<or> semantics (gs,g) e (Neg i v)")
-      apply(erule disjE) apply(rule_tac x="Pos i v" in exI) apply(force) apply(force)
-    apply(simp add: Let_def) 
-    
+     apply (metis semantics.simps(1) semantics.simps(2))
+       -- "base case, is axiom, starts with Neg"
+    apply (metis semantics.simps(1) semantics.simps(2))
+   
     -- "base case, not is axiom: if not a satax, then inference holds... but this can't be"
-   apply(drule_tac calculation_upwards) apply(assumption) apply(elim conjE exE) apply(force) 
+   apply (meson calculation_upwards le_SucI le_antisym n_not_Suc_n)
    
      -- "step case, by case analysis"
-  apply(intro allI impI) apply(elim exE conjE)
+  apply(intro allI impI)
+  apply(elim exE conjE)
 
   apply(case_tac "is_axiom (list_sequent t)")
     -- "step case, is axiom"
-  apply(simp add: valid_def) apply(rule,rule) apply(rename_tac gs g) apply(rule) apply(rule) apply(simp add: semantics_alternative_def2)
-    apply(simp add: list_sequent_def) apply(case_tac t) apply(simp) apply(simp)
-    apply(erule disjE)
-     apply(elim conjE exE)
-     apply(subgoal_tac "semantics (gs,g) e (Pos i v) \<or> semantics (gs,g) e (Neg i v)")
-      apply(erule disjE) apply(force) apply(rule_tac x="Neg i v" in exI) apply(blast)
-     apply(simp add: Let_def)
-    apply(elim conjE exE)
-    apply(subgoal_tac "semantics (gs,g) e (Pos i v) \<or> semantics (gs,g) e (Neg i v)")
-      apply(erule disjE) apply(rule_tac x="Pos i v" in exI) apply(blast) apply(simp) apply(force)
-    apply(simp add: Let_def)
-     -- "we hit Uni/ Exi cases first"
-    apply(case_tac "\<exists>(a::nat) f list. t = (a,Uni f) # list")
-   apply(elim exE) apply(simp)
-   apply(subgoal_tac "a = 0")
-    prefer 2 
-    apply(rule_tac n=na and u=t and A="Uni f" in index0[rule_format])
-    apply(assumption) apply(simp) apply(simp) apply(simp)
-   apply(frule_tac calculation.step) apply(simp add: Let_def)  -- "nice use of simp to instantiate"
-   apply(drule_tac x="Suc na" in spec, drule_tac x="list @ [(0, substitution_bind f (fresh ((flatten \<circ> map fv) (list_sequent t))))]" in spec) apply(erule impE, simp)
-   apply(subgoal_tac "fresh ((flatten \<circ> map fv)(list_sequent t)) \<notin> set ((flatten \<circ> map fv) (list_sequent t))") 
-    prefer 2 apply(rule fresh)
+   apply(simp add: valid_def)
+   apply(rule allI, rule allI)
+   apply(rename_tac gs g)
+   apply(rule allI)
+   apply(rule impI)
+   apply(simp add: semantics_alternative_def2 list_sequent_def)
+   apply(case_tac t)
+    apply(simp)
    apply(simp)
-   apply(simp add: list_sequent_def inference_def)
-   apply(frule_tac sound_FAll) apply(simp) apply(simp)
+   apply(erule disjE)
+    apply (metis semantics.simps(1) semantics.simps(2))
+   apply (metis semantics.simps(1) semantics.simps(2))
+   -- "we hit Uni/ Exi cases first"
+  apply(case_tac "\<exists>(a::nat) f list. t = (a,Uni f) # list")
+   apply(elim exE)
+   apply(simp)
+   apply(subgoal_tac "a = 0")
+    prefer 2
+    apply(rule_tac n=na and u=t and A="Uni f" in index0[rule_format])
+       apply(assumption)
+      apply(simp)
+     apply(simp)
+    apply(simp)
+   apply(frule calculation.step)
+    apply(simp)
+   apply(drule_tac x="Suc na" in spec, drule_tac x="list @ [(0, substitution_bind f (fresh ((flatten \<circ> map fv) (list_sequent t))))]" in spec)
+   apply(erule impE)
+    apply(simp)
+   using fresh list_sequent_def sound_FAll apply fastforce
   
   apply(case_tac "\<exists>a f list. t = (a,Exi f) # list")
    apply(elim exE)
-   apply(frule_tac calculation.step) apply(simp add: Let_def) -- "nice use of simp to instantiate"
-   apply(drule_tac x="Suc na" in spec, drule_tac x="list @ [(0, substitution_bind f a), (Suc a, Exi f)]" in spec) apply(erule impE, assumption)
-   apply(drule_tac x="Suc na" in spec, drule_tac x="list @ [(0, substitution_bind f a), (Suc a, Exi f)]" in spec) apply(erule impE) apply(rule) apply(arith) apply(assumption)
+   apply(frule calculation.step)
+    apply(simp)
+   apply(drule_tac x="Suc na" in spec, drule_tac x="list @ [(0, substitution_bind f a), (Suc a, Exi f)]" in spec)
+   apply(erule impE)
+    apply(assumption)
+   apply(drule_tac x="Suc na" in spec, drule_tac x="list @ [(0, substitution_bind f a), (Suc a, Exi f)]" in spec)
+   apply(erule impE)
+    apply(simp)
    apply(subgoal_tac "valid (list_sequent (list@[(0,substitution_bind f a), (Suc a, Exi f)]))")
-    apply(simp add: list_sequent_def)
-    apply(frule_tac sound_FEx) apply(simp) apply(simp)
+    apply (simp add: list_sequent_def sound_FEx)
+   apply(simp)
   -- "now for other cases"
       -- "case empty list"
-  apply(case_tac t) apply(simp)
-   apply(frule_tac step) apply(simp) apply(simp) apply(metis add_Suc_shift add_right_cancel diff_add)
+  apply(case_tac t)
+   apply(frule step)
+    apply(simp)
+   apply(metis add_Suc_shift add_right_cancel diff_add)
    
-  apply(simp add: valid_def) apply(rule,rule) apply(rename_tac gs g) apply(rule) apply(rule) apply(simp add: semantics_alternative_def2)
+  apply(simp add: valid_def semantics_alternative_def2)
+  apply(rule allI, rule allI)
+  apply(rename_tac gs g)
+  apply(rule allI)
+  apply(rule impI)
   -- "na t in calculation, so too is inference"
    -- "if not a satax, then inference holds... "
   apply(case_tac a)
   apply(case_tac b)
-       apply(simp del: semantics.simps) apply(frule_tac patom) apply(assumption)
+       apply(simp del: semantics.simps)
+       apply(frule patom)
+        apply(assumption)
        apply(rename_tac nat lista)
        apply(frule_tac x="Suc na" in spec, drule_tac x="list @ [(0, Pos nat lista)]" in spec)
-       apply(erule impE) apply(arith)
-       apply(drule_tac x=gs in spec, drule_tac x=g in spec, drule_tac x=e in spec) apply(erule impE) apply(simp add: is_model_environment_def)
-       apply(elim exE conjE) apply(rule_tac x=p in exI) apply(simp add: list_sequent_def) -- "weirdly, simp succeeds, force and blast fail"
-     apply(simp del: semantics.simps) apply(frule_tac fconj1) apply(assumption) apply(frule_tac fconj2) apply(assumption)
-     apply(rename_tac form1 form2)
-     apply(frule_tac x="Suc na" in spec, drule_tac x="list @ [(0, form1)]" in spec)
-     apply(erule impE) apply(arith)
-     apply(drule_tac x=gs in spec, drule_tac x=g in spec, drule_tac x=e in spec) apply(erule impE, simp) apply(elim exE conjE)
-     apply(drule_tac x="Suc na" in spec, drule_tac x="list @ [(0, form2)]" in spec)
-     apply(erule impE) apply(arith)
-     apply(drule_tac x=gs in spec, drule_tac x=g in spec, drule_tac x=e in spec) apply(erule impE, simp) apply(elim exE conjE)
-     apply(simp only: list_sequent_def) 
+       apply(erule impE)
+        apply(simp)
+       apply(drule_tac x=gs in spec, drule_tac x=g in spec, drule_tac x=e in spec)
+       apply(erule impE)
+        apply(simp add: is_model_environment_def)
+       apply(elim exE conjE)
+       apply(rule_tac x=p in exI)
+       apply(simp add: list_sequent_def)
+      apply(simp del: semantics.simps)
+      apply(frule_tac fconj1)
+       apply(assumption)
+      apply(frule_tac fconj2)
+       apply(assumption)
+      apply(rename_tac form1 form2)
+      apply(frule_tac x="Suc na" in spec, drule_tac x="list @ [(0, form1)]" in spec)
+      apply(erule impE)
+       apply(arith)
+      apply(drule_tac x=gs in spec, drule_tac x=g in spec, drule_tac x=e in spec)
+      apply(erule impE)
+       apply(simp)
+      apply(elim exE conjE)
+      apply(drule_tac x="Suc na" in spec, drule_tac x="list @ [(0, form2)]" in spec)
+      apply(erule impE)
+       apply(simp)
+      apply(drule_tac x=gs in spec, drule_tac x=g in spec, drule_tac x=e in spec)
+      apply(erule impE)
+       apply(simp)
+      apply(elim exE conjE)
+      apply(simp add: list_sequent_def)
+      apply(auto)[1]
+     apply(fastforce)
+    apply(simp del: semantics.simps)
+    apply(frule natom)
+     apply(assumption)
+    apply(rename_tac nat lista)
+    apply(frule_tac x="Suc na" in spec, drule_tac x="list @ [(0, Neg nat lista)]" in spec)
+    apply(erule impE)
      apply(simp)
-     apply(elim disjE) 
-        apply(simp) apply(rule_tac x="Con form1 form2" in exI) apply(simp)
-       apply(simp) apply(rule_tac x="pa" in exI) apply(simp)
-      apply(simp) apply(rule_tac x="p" in exI) apply(simp)
-     apply(rule_tac x="p" in exI, simp)
-   apply(force)
-      apply(simp del: semantics.simps) apply(frule_tac natom) apply(assumption)
-      apply(rename_tac nat lista)
-      apply(frule_tac x="Suc na" in spec, drule_tac x="list @ [(0, Neg nat lista)]" in spec)
-      apply(erule impE) apply(arith)
-      apply(drule_tac x=gs in spec, drule_tac x=g in spec, drule_tac x=e in spec) apply(erule impE, simp)
-      apply(elim exE conjE) apply(rule_tac x=p in exI) apply(simp add: list_sequent_def)
-    apply(simp del: semantics.simps) apply(frule_tac fdisj) apply(assumption)
-    apply(rename_tac form1 form2)
-    apply(frule_tac x="Suc na" in spec, drule_tac x="list @ [(0, form1),(0,form2)]" in spec)
-    apply(erule impE) apply(simp)
-    apply(drule_tac x=gs in spec, drule_tac x=g in spec, drule_tac x=e in spec) apply(erule impE, simp) apply(elim exE conjE)
+    apply(drule_tac x=gs in spec, drule_tac x=g in spec, drule_tac x=e in spec)
+    apply(erule impE)
+     apply(simp)
+    apply(elim exE conjE)
+    apply(rule_tac x=p in exI)
     apply(simp add: list_sequent_def)
-    apply(elim disjE)
-      apply(simp) apply(rule_tac x="Dis form1 form2" in exI) apply(simp)
-     apply(simp) apply(rule_tac x="Dis form1 form2" in exI) apply(simp)
-    apply(rule_tac x="p" in exI) apply(simp)
-      -- "all case"
-  apply(force)
+   apply(simp del: semantics.simps)
+   apply(frule_tac fdisj)
+    apply(assumption)
+   apply(rename_tac form1 form2)
+   apply(frule_tac x="Suc na" in spec, drule_tac x="list @ [(0, form1),(0,form2)]" in spec)
+   apply(erule impE)
+    apply(simp)
+   apply(drule_tac x=gs in spec, drule_tac x=g in spec, drule_tac x=e in spec)
+   apply(erule impE)
+    apply(simp)
+   using list_sequent_def snd_eqD apply auto[1]
+  -- "all case"
+  apply(blast)
   done
 
 lemma xxx[simp]: "list_sequent (make_sequent s) = s"
-  by (induct s) (simp_all add: list_sequent_def make_sequent_def)
+  using list_sequent_def make_sequent_def by (induct s) simp_all
 
-lemma soundness: "finite (calculation (make_sequent s)) \<Longrightarrow> valid s"
-  apply(subgoal_tac "init (make_sequent s)") 
-   prefer 2 apply(simp add: init_def make_sequent_def)
-  apply(subgoal_tac "finite (fst ` (calculation (make_sequent s)))") prefer 2 apply(simp)
-  apply(frule_tac max_exists) apply(erule impE) apply(simp) apply(subgoal_tac "(0,make_sequent s) \<in> calculation (make_sequent s)") apply(force) apply(simp)
-  apply(elim exE conjE)
-  apply(frule_tac soundness') apply(assumption) apply(assumption) apply(force) 
-  apply(drule_tac x=0 in spec, drule_tac x="make_sequent s" in spec)
-  apply(force)
-  done
+lemma soundness:
+  assumes 1: "finite (calculation (make_sequent s))"
+  shows "valid s"
+  proof -
+    have "init (make_sequent s)" and "finite (fst ` (calculation (make_sequent s)))"
+      using 1 by (simp add: init_def make_sequent_def, simp)
+    then show ?thesis using 1 calculation.init soundness' xxx max_exists
+      by (metis (mono_tags, lifting) empty_iff fst_conv image_eqI)
+qed
 
 section "Contains / Considers"
 
@@ -563,202 +561,216 @@ definition contains :: "(nat \<Rightarrow> (nat \<times> sequent)) \<Rightarrow>
 definition considers :: "(nat \<Rightarrow> (nat \<times> sequent)) \<Rightarrow> nat \<Rightarrow> nat \<times> form \<Rightarrow> bool" where
   "considers f n nf = (case snd (f n) of [] \<Rightarrow> False | (x # xs) \<Rightarrow> x = nf)"
 
-lemma (in loc1) progress: "infinite (calculation s) \<Longrightarrow> snd (f n) = a # list \<longrightarrow> (\<exists>zs'. snd (f (Suc n)) = list@zs')"
-using inference_def apply(subgoal_tac "(snd (f (Suc n))) : set (inference (snd (f n)))") defer apply(frule_tac is_path_f) apply(blast)
-  apply(case_tac a)
-  apply(case_tac b)
-  apply(safe)
-  apply(simp_all add: split: if_splits)
-  apply(erule disjE)
-  apply(simp_all)
-  done
+lemma (in loc1) progress:
+  assumes 1: "infinite (calculation s)"
+  shows "snd (f n) = a # list \<longrightarrow> (\<exists>zs'. snd (f (Suc n)) = list@zs')"
+  proof -
+    obtain 2: "(snd (f (Suc n))) : set (inference (snd (f n)))" using 1 is_path_f by blast
+    then show ?thesis proof (cases a)
+      case (Pair _ b)
+      then show ?thesis using 2 inference_def
+        by (induct b, safe, simp_all split: if_splits) blast
+  qed
+qed
 
-lemma (in loc1) contains_considers': "infinite (calculation s) \<Longrightarrow> \<forall>n y ys. snd (f n) = xs@y # ys \<longrightarrow> (\<exists>m zs'. snd (f (n+m)) = y # zs')"
-  apply(induct_tac xs)
-  apply(rule,rule,rule,rule) apply(rule_tac x=0 in exI) apply(rule_tac x=ys in exI) apply(force)
-
-  apply(rule,rule,rule,rule) apply(simp) apply(frule_tac progress) apply(erule impE) apply(assumption)
-  apply(erule exE) apply(simp) 
-
+lemma (in loc1) contains_considers'[rule_format]: "infinite (calculation s) \<Longrightarrow> \<forall>n y ys. snd (f n) = xs@y # ys \<longrightarrow> (\<exists>m zs'. snd (f (n+m)) = y # zs')"
+  apply(induct xs)
+   apply(simp)
+   apply (metis Nat.add_0_right)
+  
+  apply(rule allI, rule allI, rule allI, rule impI)
+  apply(simp)
+  apply(frule progress)
+  apply(erule impE)
+   apply(assumption)
+  apply(erule exE)
+ 
   apply(drule_tac x="Suc n" in spec)
-  apply(case_tac y) apply(rename_tac u v)
+  apply(case_tac y)
+  apply(rename_tac u v)
   apply(drule_tac x="u" in spec)
   apply(drule_tac x="v" in spec)
-  apply(erule impE) apply(force)
+  apply(erule impE)
+   apply(simp)
   
-  apply(elim exE)
-  apply(rule_tac x="Suc m" in exI)
-  apply(force)
+  apply(metis add_Suc_shift)
   done
 
 lemma list_decomp[rule_format]: "v \<in> set p \<longrightarrow> (\<exists>xs ys. p = xs@(v # ys) \<and> v \<notin> set xs)"
-  apply(induct p)
-  apply(force)
-  apply(case_tac "v=a")
-   apply(force)
-  apply(auto)
-  apply(rule_tac x="a # xs" in exI)
-  apply(auto)
-  done
-
+  by (meson split_list_first)
+ 
 lemma (in loc1) contains_considers: "infinite (calculation s) \<Longrightarrow> contains f n y \<Longrightarrow> (\<exists>m. considers f (n+m) y)"
-  apply(simp add: contains_def considers_def)
-  apply(frule_tac list_decomp) apply(elim exE conjE)
-  apply(frule_tac contains_considers'[rule_format]) apply(assumption) apply(elim exE)
-  apply(rule_tac x=m in exI)
-  apply(force)
-  done
+  by (simp add: contains_def, frule list_decomp, elim exE conjE, frule contains_considers')
+     (assumption, metis (mono_tags, lifting) considers_def list.simps(5))
 
 lemma (in loc1) contains_propagates_patoms[rule_format]: "infinite (calculation s) \<Longrightarrow> contains f n (0, Pos i v) \<longrightarrow> contains f (n+q) (0, Pos i v)"
-using inference_def apply(induct_tac q) apply(simp)
-  apply(rule)
-  apply(erule impE) apply(assumption)
+  using inference_def
+  apply(induct_tac q)
+   apply(simp)
+  apply(rule impI)
+  apply(erule impE)
+   apply(assumption)
   apply(subgoal_tac "\<not> is_axiom (list_sequent (snd (f (n+na))))") defer
    apply(subgoal_tac "infinite (calculation (snd (f (n+na))))") defer
-    apply(force dest: is_path_f)
-   defer
-   apply(rule) apply(simp add: calculation_is_axiom)
+    apply(fastforce dest: is_path_f) defer
+   apply(rule notI)
+   apply(simp add: calculation_is_axiom)
   apply(simp add: contains_def)
   apply(drule_tac p="snd (f (n + na))" in list_decomp) 
   apply(elim exE conjE)
   apply(case_tac xs)
-   apply(simp)
    apply(subgoal_tac "(snd (f (Suc (n + na)))) : set (inference (snd (f (n + na))))")
-    apply(simp add: split: if_splits)
-   apply(frule_tac is_path_f) apply(drule_tac x="n+na" in spec) apply(force)
-  apply(drule_tac progress)
-  apply(erule impE) apply(force)
-  apply(force)
+    apply(simp split: if_splits)
+   apply(frule is_path_f)
+   apply(drule_tac x="n+na" in spec)
+   apply(simp)
+  apply(drule progress)
+  apply(erule impE)
+   apply(simp)
+  apply(clarsimp)
   done
 
 lemma (in loc1) contains_propagates_natoms[rule_format]: "infinite (calculation s) \<Longrightarrow> contains f n (0, Neg i v) \<longrightarrow> contains f (n+q) (0, Neg i v)"
-using inference_def apply(induct_tac q) apply(simp)
-  apply(rule)
-  apply(erule impE) apply(assumption)
+  using inference_def
+  apply(induct_tac q)
+   apply(simp)
+  apply(rule impI)
+  apply(erule impE)
+   apply(assumption)
   apply(subgoal_tac "\<not> is_axiom (list_sequent (snd (f (n+na))))") defer
    apply(subgoal_tac "infinite (calculation (snd (f (n+na))))") defer
-    apply(force dest: is_path_f)
-   defer
-   apply(rule) apply(simp add: calculation_is_axiom)
+    apply(fastforce dest: is_path_f) defer
+   apply(rule notI)
+   apply(simp add: calculation_is_axiom)
   apply(simp add: contains_def)
   apply(drule_tac p = "snd (f (n + na))" in list_decomp) 
   apply(elim exE conjE)
   apply(case_tac xs)
    apply(simp)
    apply(subgoal_tac "(snd (f (Suc (n + na)))) : set (inference (snd (f (n + na))))")
-    apply(simp add: split: if_splits)
-   apply(frule_tac is_path_f) apply(drule_tac x="n+na" in spec) apply(force)
+    apply(simp split: if_splits)
+   apply(frule_tac is_path_f)
+   apply(drule_tac x="n+na" in spec)
+   apply(simp)
   apply(drule_tac progress)
-  apply(erule impE) apply(force)
-  apply(force)
+  apply(erule impE)
+   apply(simp)
+  apply(clarsimp)
   done
 
 lemma (in loc1) contains_propagates_fconj: "infinite (calculation s) \<Longrightarrow> contains f n (0, Con g h) \<Longrightarrow> (\<exists>y. contains f (n+y) (0,g) \<or> contains f (n+y) (0,h))"
-  apply(subgoal_tac "(\<exists>l. considers f (n+l) (0,Con g h))") defer apply(rule contains_considers) apply(assumption) apply(assumption)
+  apply(subgoal_tac "(\<exists>l. considers f (n+l) (0,Con g h))") defer
+   apply(rule contains_considers)
+    apply(assumption)
+   apply(assumption)
   apply(erule exE)
   apply(rule_tac x="Suc l" in exI)
-  apply(simp add: considers_def) apply(case_tac "snd (f (n + l))", simp)
-  apply(simp)
+  apply(simp add: considers_def)
+  apply(case_tac "snd (f (n + l))")
+   apply(simp)
   apply(subgoal_tac "(snd (f (Suc (n + l)))) : set (inference (snd (f (n + l))))")
-   apply(simp add: contains_def inference_def) apply(force)
-  apply(frule_tac is_path_f) apply(drule_tac x="n+l" in spec) apply(force)
+   apply(fastforce simp: contains_def inference_def)
+  apply(frule_tac is_path_f)
+  apply(drule_tac x="n+l" in spec)
+  apply(simp)
   done
 
 lemma (in loc1) contains_propagates_fdisj: "infinite (calculation s) \<Longrightarrow> contains f n (0, Dis g h) \<Longrightarrow> (\<exists>y. contains f (n+y) (0,g) \<and> contains f (n+y) (0,h))"
-  apply(subgoal_tac "(\<exists>l. considers f (n+l) (0,Dis g h))") defer apply(rule contains_considers) apply(assumption) apply(assumption)
+  apply(subgoal_tac "(\<exists>l. considers f (n+l) (0,Dis g h))")
+   defer
+   apply(rule contains_considers)
+    apply(assumption)
+   apply(assumption)
   apply(erule exE)
   apply(rule_tac x="Suc l" in exI)
-  apply(simp add: considers_def) apply(case_tac "snd (f (n + l))", simp)
-  apply(simp)
+  apply(simp add: considers_def)
+  apply(case_tac "snd (f (n + l))")
+   apply(simp)
   apply(subgoal_tac " (snd (f (Suc (n + l)))) : set (inference (snd (f (n + l))))")
    apply(simp add: contains_def inference_def) 
-  apply(frule_tac is_path_f) apply(drule_tac x="n+l" in spec) apply(force)
+  apply(frule_tac is_path_f)
+  apply(drule_tac x="n+l" in spec)
+  apply(simp)
   done
 
 lemma (in loc1) contains_propagates_fall: "infinite (calculation s) \<Longrightarrow> contains f n (0, Uni g)
   \<Longrightarrow> (\<exists>y. contains f (Suc(n+y)) (0,substitution_bind g (fresh (fv_list (list_sequent (snd (f (n+y))))))))" -- "may need constraint on fv"
 using fv_list_def
-  apply(subgoal_tac "(\<exists>l. considers f (n+l) (0,Uni g))") defer apply(rule contains_considers) apply(assumption) apply(assumption)
+  apply(subgoal_tac "(\<exists>l. considers f (n+l) (0,Uni g))") defer
+   apply(rule contains_considers)
+    apply(assumption)
+   apply(assumption)
   apply(erule exE)
   apply(rule_tac x="l" in exI)
-  apply(simp add: considers_def) apply(case_tac "snd (f (n + l))", simp)
-  apply(simp)
+  apply(simp add: considers_def)
+  apply(case_tac "snd (f (n + l))")
+   apply(simp)
   apply(subgoal_tac "(snd (f (Suc (n + l)))) : set (inference (snd (f (n + l))))")
    apply(simp add: contains_def inference_def)
-  apply(frule_tac is_path_f) apply(drule_tac x="n+l" in spec) apply(force)
+  apply(frule_tac is_path_f)
+  apply(drule_tac x="n+l" in spec)
+  apply(simp)
   done
 
 lemma (in loc1) contains_propagates_fex: "infinite (calculation s) \<Longrightarrow> contains f n (m, Exi g) 
   \<Longrightarrow> (\<exists>y. (contains f (n+y) (0,substitution_bind g m)) \<and> (contains f (n+y) (Suc m,Exi g)))"
-  apply(subgoal_tac "(\<exists>l. considers f (n+l) (m,Exi g))") defer apply(rule contains_considers) apply(assumption) apply(assumption)
+  apply(subgoal_tac "(\<exists>l. considers f (n+l) (m,Exi g))") defer
+   apply(rule contains_considers)
+    apply(assumption)
+   apply(assumption)
   apply(erule exE)
   apply(rule_tac x="Suc l" in exI)
-  apply(simp add: considers_def) apply(case_tac "snd (f (n + l))", simp)
-  apply(simp)
+  apply(simp add: considers_def)
+  apply(case_tac "snd (f (n + l))")
+   apply(simp)
   apply(subgoal_tac " (snd (f (Suc (n + l)))) : set (inference (snd (f (n + l))))")
    apply(simp add: contains_def inference_def)
-  apply(frule_tac is_path_f) apply(drule_tac x="n+l" in spec) apply(force)
+  apply(frule_tac is_path_f)
+  apply(drule_tac x="n+l" in spec)
+  apply(simp)
   done
 
   -- "also need that if contains one, then contained an original at beginning"
   -- "existentials: show that for exists formulae, if Suc m is marker, then there must have been m"
   -- "show this by showing that nodes are upwardly closed, i.e. if never contains (m,x), then never contains (Suc m, x), by induction on n"
 
-lemma (in loc1) FEx_downward: "infinite (calculation s) \<Longrightarrow> init s \<Longrightarrow> \<forall>m. (Suc m,Exi g) \<in> set (snd (f n)) \<longrightarrow> (\<exists>n'. (m, Exi g) \<in> set (snd (f n')))"
-using inference_def apply(frule_tac is_path_f)
+lemma (in loc1) FEx_downward: "infinite (calculation s) \<Longrightarrow> init s \<Longrightarrow> \<forall>m. (Suc m, Exi g) \<in> set (snd (f n)) \<longrightarrow> (\<exists>n'. (m, Exi g) \<in> set (snd (f n')))"
+  using inference_def
+  apply(frule_tac is_path_f)
   apply(induct_tac n)
-   apply(drule_tac x="0" in spec) apply(case_tac "f 0") apply(force simp: init_def) 
+   apply(drule_tac x="0" in spec)
+   apply(case_tac "f 0")
+   apply(force simp: init_def) 
   apply(intro allI impI)
-  apply(frule_tac x="Suc n" in spec, elim conjE) apply(drule_tac x="n" in spec, elim conjE)
+  apply(frule_tac x="Suc n" in spec)
+  apply(drule_tac x="n" in spec, elim conjE)
   apply(thin_tac "(snd (f (Suc (Suc n)))) : set (inference (snd (f (Suc n))))")
-  apply(case_tac "f n") apply(simp)
-  apply(case_tac b) apply(simp)
-  apply(case_tac aa) apply(case_tac ba)
-       apply(simp add: split: if_splits)
-     apply(force simp add: Let_def)
-    apply(force simp add: Let_def)
-      apply(simp add: split: if_splits)
-   apply(force simp add: Let_def)
+  apply(case_tac "f n")
+  apply(case_tac b)
+   apply(simp)
+  apply(case_tac aa)
+  apply(case_tac ba)
+       apply(simp split: if_splits)
+      apply(fastforce)
+     apply(fastforce)
+    apply(simp split: if_splits)
+   apply(fastforce)
   apply(rename_tac form)
   apply(case_tac "(ab, Exi form) = (m, Exi g)")
-   apply(rule_tac x=n in exI) apply(force)
-  apply(auto simp add: Let_def)
+   apply(rule_tac x=n in exI)
+   apply(simp)
+  apply(auto)
   done
    
 lemma (in loc1) FEx0: "infinite (calculation s) \<Longrightarrow> init s \<Longrightarrow> \<forall>n. contains f n (m,Exi g) \<longrightarrow> (\<exists>n'. contains f n' (0, Exi g))"
-  apply(simp add: contains_def)
-  apply(induct_tac m)
-   apply(force)
-  apply(intro allI impI) apply(erule exE) 
-  apply(drule_tac FEx_downward[rule_format]) apply(assumption) apply(force)
-  apply(elim exE conjE)
-  apply(force)
-  done
+  using FEx_downward contains_def by (induct_tac m) (simp, blast)
      
 lemma (in loc1) FEx_upward': "infinite (calculation s) \<Longrightarrow> init s \<Longrightarrow> \<forall>n. contains f n (0, Exi g) \<longrightarrow> (\<exists>n'. contains f n' (m, Exi g))"
-  apply(intro allI impI)
-  apply(induct_tac m) apply(force)
-  apply(erule exE)
-  apply(frule_tac n=n' in contains_considers) apply(assumption) 
-  apply(erule exE)
-  apply(rule_tac x="Suc(n'+m)" in exI)
-  apply(frule_tac is_path_f) 
-  apply(simp add: considers_def) apply(case_tac "snd (f (n'+m))") apply(force)
-  apply(simp)
-  apply(drule_tac x="n'+m" in spec)
-  apply(force simp add: contains_def considers_def inference_def)
-  done -- "FIXME contains and considers aren't buying us much"
+  using contains_propagates_fex by (induct_tac m) (simp, blast)
 
 lemma (in loc1) FEx_upward: "infinite (calculation s) \<Longrightarrow> init s \<Longrightarrow> contains f n (m, Exi g) \<Longrightarrow> (\<forall>m'. \<exists>n'. contains f n' (0, substitution_bind g m'))"
-using inference_def apply(intro allI impI)
-  apply(subgoal_tac "\<exists>n'. contains f n' (m', Exi g)") defer
-  apply(frule_tac m = m and g = g in FEx0) apply(assumption)
-  apply(drule_tac x=n in spec)
-  apply(simp)
-  apply(elim exE)
-  apply(frule_tac g=g and m=m' in FEx_upward') apply(assumption)
-  apply (blast dest: contains_propagates_fex intro: elim:)+
-  done
+  using contains_propagates_fex FEx0 FEx_upward'
+  by (intro allI, subgoal_tac "\<exists>n'. contains f n' (m', Exi g)") (blast, blast)
 
 abbreviation ntou :: "nat \<Rightarrow> proxy" where "ntou \<equiv> id"
 
@@ -784,7 +796,6 @@ lemma size_substitution_bind[simp]: "size (substitution_bind f m) = size f"
   using substitution_bind_def by simp
 
 lemma (in loc2) model': "infinite (calculation s) \<Longrightarrow> init s \<Longrightarrow> \<forall>A. size A = h \<longrightarrow> (\<forall>m n. contains f n (m,A) \<longrightarrow> \<not> (semantics mo ntou A))"
-
   apply(rule_tac nat_less_induct) apply(rule, rule) apply(case_tac A) 
        apply(rule,rule,rule) apply(simp add: mo Let_def) apply(simp add: model_def Let_def) apply(simp only: f[symmetric]) apply(force)
 
@@ -838,39 +849,22 @@ lemma (in loc2) model': "infinite (calculation s) \<Longrightarrow> init s \<Lon
   done
    
 lemma (in loc2) model: "infinite (calculation s) \<Longrightarrow> init s \<Longrightarrow> (\<forall>A m n. contains f n (m,A) \<longrightarrow> \<not> (semantics mo ntou A))"
-  by (simp add: model')
+  using model' by simp
 
 section "Completeness"
 
 lemma (in loc2) completeness': "infinite (calculation s) \<Longrightarrow> init s \<Longrightarrow> \<forall>mA \<in> set s. \<not> semantics mo ntou (snd mA)" -- "FIXME tidy calculation s so that s consists of formulae only?"
-  apply(frule_tac model) apply(assumption)
-  apply(rule)
-  apply(case_tac mA)
-  apply(drule_tac x="b" in spec) apply(drule_tac x="0" in spec) apply(drule_tac x=0 in spec) apply(erule impE)
-   apply(simp add: contains_def) apply(frule_tac is_path_f_0) apply(simp) 
-   apply(subgoal_tac "a=0") 
-    prefer 2 apply(simp only: init_def, force)
-  apply auto
-  done -- "FIXME very ugly"
-
+  by (metis SimPro.contains_def eq_snd_iff is_path_f_0 model)
+ 
 lemma completeness': "infinite (calculation s) \<Longrightarrow> init s \<Longrightarrow> \<forall>mA \<in> set s. \<not> semantics (model s) ntou (snd mA)"
   by (rule loc2.completeness'[simplified loc2_def loc2_axioms_def loc1_def]) simp
 
 lemma completeness'': "infinite (calculation (make_sequent s)) \<Longrightarrow> init (make_sequent s) \<Longrightarrow> \<forall>A. A \<in> set s \<longrightarrow> \<not> semantics (model (make_sequent s)) ntou A"
-  using completeness' make_sequent_def by force
+  using completeness' make_sequent_def by fastforce
 
 lemma completeness: "infinite (calculation (make_sequent s)) \<Longrightarrow> \<not> valid s"
-  apply(subgoal_tac "init (make_sequent s)") 
-   prefer 2 apply(simp add: init_def make_sequent_def)
-  apply(frule_tac completeness'') apply(assumption)
-  apply(simp add: valid_def)
-  apply(simp add: semantics_alternative_def2)
-  apply(rule_tac x="fst (model (make_sequent s))" in exI)
-  apply(rule_tac x="snd (model (make_sequent s))" in exI)
-  apply(rule_tac x="ntou" in exI)
-  apply(simp add: model_def)
-  apply(simp add: is_model_environment_def)
-  done -- "FIXME silly splitting of quantified pairs "
+  using valid_def init_def make_sequent_def is_env_model_ntou semantics_alternative_def2 completeness''
+  by(subgoal_tac "init (make_sequent s)") (metis, simp)
 
 section "Algorithm"
 
@@ -878,7 +872,7 @@ definition loop :: "sequent list \<Rightarrow> nat \<Rightarrow> sequent list" w
   "loop s n = repeat (flatten \<circ> map inference) s n"
 
 lemma loop_upwards: "loop s n = [] \<Longrightarrow> loop s (n+m) = []"
-  by (induct m) (auto simp add: loop_def)
+  using loop_def by (induct m) auto
 
 lemma flatten_append: "flatten (xs@ys) = ((flatten xs) @ (flatten ys))"
   by (induct xs) auto
@@ -888,45 +882,55 @@ lemma set_flatten: "set (flatten xs) = Union (set ` set xs)"
 
 lemma loop: "\<forall>x. ((n,x) \<in> calculation s) = (x \<in> set (loop [s] n))"
   apply(induct n)
-  apply(simp) apply(simp add: loop_def)
-  apply(rule)
-  apply(rule)
-   apply(drule_tac calculation_downwards)
+   apply(simp add: loop_def)
+  apply(rule allI)
+  apply(rule iffI)
+   apply(drule calculation_downwards)
    apply(elim exE conjE)
    apply(drule_tac x=y in spec)
    apply(simp)
-   apply(drule_tac list_decomp) apply(elim exE conjE)
-   apply(simp add: flatten_append loop_def Let_def)
-  apply(simp add: loop_def)
-  apply(simp add: set_flatten)
-  apply(erule bexE)
-  apply(drule_tac x=a in spec)
-  apply(rule step) apply(auto)
+   apply(drule list_decomp)
+   apply(elim exE conjE)
+   apply(simp add: flatten_append loop_def)
+  apply(simp add: loop_def set_flatten)
+  apply(blast)
   done
 
 lemma calculation_f: "calculation s = UNION UNIV (\<lambda>x. set (map (\<lambda>y. (x,y)) (loop [s] x)))"
-  by (force simp add: loop)  
+  using loop by fastforce
 
 lemma finite_calculation: "finite (calculation s) = (\<exists>m. loop [s] m = [])"
-  apply(rule)
+  apply(rule iffI)
    apply(subgoal_tac "finite (fst ` (calculation s))") prefer 2 apply(simp)
-   apply(frule_tac max_exists) apply(erule impE) apply(simp) apply(subgoal_tac "(0,s) \<in> calculation s") apply(force) apply(simp)
+   apply(frule max_exists)
+   apply(erule impE)
+    apply(subgoal_tac "(0,s) \<in> calculation s")
+     apply(fastforce)
+    apply(simp)
    apply(elim exE conjE)
    apply(rule_tac x="Suc x" in exI)
-   apply(simp)
-   apply(rule ccontr) apply(case_tac "loop [s] (Suc x)") apply(simp) 
-   apply(subgoal_tac "(Suc x, a) \<in> calculation s") apply(force)
+   apply(rule ccontr)
+   apply(case_tac "loop [s] (Suc x)")
+    apply(simp) 
+   apply(subgoal_tac "(Suc x, a) \<in> calculation s")
+    apply(fastforce)
    apply(simp add: loop)
   apply(erule exE)
   apply(subgoal_tac "\<forall>y. loop [s] (m+y) = []") 
-   prefer 2 apply(rule) apply(rule loop_upwards) apply(assumption)
+   prefer 2 apply(rule allI)
+   apply(rule loop_upwards)
+   apply(assumption)
   apply(simp add: calculation_f)
   apply(subgoal_tac "(UNIV::nat set) = {y. y < m} Un {y. m \<le> y}")
-   prefer 2 apply force
+   prefer 2 apply fastforce
   apply(erule_tac t="UNIV::nat set" in ssubst) 
   apply(simp)
-  apply(subgoal_tac "(UN x:Collect (op \<le> m). Pair x ` set (loop [s] x)) =  (UN x:Collect (op \<le> m). {})") apply(simp only:) apply(force)
-  apply(rule SUP_cong) apply(force) apply(drule_tac x="x-m" in spec) apply(force)
+  apply(subgoal_tac "(UN x:Collect (op \<le> m). Pair x ` set (loop [s] x)) =  (UN x:Collect (op \<le> m). {})")
+   apply(simp)
+  apply(rule SUP_cong)
+   apply(simp)
+  apply(drule_tac x="x-m" in spec)
+  apply(simp)
   done
 
 (**************************************************************************************************)
